# Aufgabenblatt 7
**Aufgabe 1**
a) $f(x) = \frac x {1 + x^2}$
$f(x)' = \frac {1 - x^2}{(1 +x^2)^2}$
b)
$f(x) = \frac {sin(x)} x$
$f'(x) = \frac{cos(x)x - sin(x)}{x^2}$
c)
$f(x) = e^{-2x}\cos(3x)$
$f'(x) = -2e^{-2x}cos(3x) + e^{-2x}sin(3x)3$
d)

$f(x) = \ln(x+\sqrt{1 + x^2})$
$u = ln(x)$ 
$u' = \frac 1 x$
$v = x + \sqrt{1+x^2}$
$v' = 1 + \frac 1 {2\sqrt{1 + x}}$
$f'(x) =\frac 1 {x + \sqrt{1+2x^2}} *(1 + \frac 1 {2\sqrt{1 + x}})$
**Prüfen!!!!**
e) $f(x) = \arctan(\frac 1 {x^2})$
$f'(x) = \arctan'(\frac{1}{x^2}) * -1{x^2}^{-2} = \arctan'(\frac{1}{x^2})*-\frac{1}{x^4}$$=\frac{1}{1+\frac{1}{x^4}}\times-\frac{1}{x^4} = - \frac{1}{x^4+1}$
**Prüfen ist falsch**

---
**Aufgabe 2**
a) $f(x) = \frac{1}{8}x^3 - \frac{3}{2}x + 2$
$f'(x) =\frac{3}{8}x^2-1.5$
Tangente bei $x_0 = 0$:
$y = 2- 1.5x$ 
Tangente bei $x_1 = 2$:
$y = f(2) + f'(2)(x-2) = 0$ 
Tangente bei $x_2 = -2$:
$y = 4$ 
**Schnittpunkte mit dingi noch berechnen**
b) $f(x) = cosh(x):= \frac{1}{2}(e^x+e^{-x}) = \frac{1}{2} e^x + \frac{1}{2}e^{-x}$
$f'(x) =\frac{1}{2}e^x - \frac{1}{2}e^{-x}$
Tangente bei $x_0 = 0$:
$y = f(0) + f'(0)x = 0$
Tangente bei $x_1 = ln(2)$:
$y = f(ln(x)) +f'(ln(2))(x-ln(2))$